\documentclass[a4paper]{article}
\usepackage{amsmath,amssymb,amsthm}
\usepackage{bm}
\usepackage{biblatex}
\usepackage{float}
\usepackage[colorlinks=true, urlcolor=cyan]{hyperref}
\usepackage{graphicx}
\usepackage{mathtools}
\usepackage{physics}

\renewcommand{\thesection}{\arabic{section}}
\renewcommand{\thesubsection}{\arabic{section}.\alph{subsection}}

\setlength{\parindent}{0pt} % Disable indentation
\mathtoolsset{showonlyrefs} % Only show equation numbers on referenced equations


\begin{document}

\hypersetup{pageanchor=false}
\begin{titlepage}
    \centering
    \vfill
    {\Large
        {\Large ELEC 442 - Introduction to Robotics\\}
        \vskip.5cm
        {\huge Assignment 1\\
        \vskip2cm
        Sondre Myrberg\\
        \href{mailto:sondrmyr@alumni.ubc.ca}{sondrmyr@alumni.ubc.ca}\\
        81113433\\}
    }
    \vfill
    \includegraphics[width=0.95\textwidth]{../../ubc_logo.pdf}
    \vfill
    \vfill
\end{titlepage}
\hypersetup{pageanchor=true}

\section{}

Given the homogenous transformation
\begin{equation}
    \begin{bmatrix}
        \bm{y} \\ 1
    \end{bmatrix} = 
    \underbrace{\begin{bmatrix}
        Q & \bm{d} \\ \bm{0}^\top & 1 
    \end{bmatrix}}_{T}
    \begin{bmatrix}
        \bm{x} \\ 1
    \end{bmatrix}
\end{equation}
where $Q$ and $\bm{d}$ accounts for rotation and translation, respectively. We have that the inverse
is given by 
\begin{equation}
        T^{-1} = \begin{bmatrix}
            \tilde{Q} & \tilde{\bm{d}} \\ \bm{0}^\top & 1
        \end{bmatrix}
\end{equation}
where we know that $T^{-1}T$ is equal to the $4\!\cross\!4$ identity matrix. This yields
\begin{equation}
    \begin{aligned}
        T^{-1}T &= \begin{bmatrix}
             \tilde{Q} & \tilde{\bm{d}} \\ \bm{0}^\top & 1
        \end{bmatrix}
        \begin{bmatrix}
            Q & \bm{d} \\ \bm{0}^\top & 1
        \end{bmatrix} \\
        &= \begin{bmatrix}
            \tilde{Q}Q & \tilde{Q}\bm{d} + \tilde{\bm{d}} \\ \bm{0}^\top & 1
        \end{bmatrix} = \mathbf{I}_{4\cross4}\\
        \implies &\begin{cases}
            \tilde{Q}Q &= \mathbf{I}_{3\cross3} \\
             \tilde{Q}\bm{d} + \tilde{\bm{d}} &= \bm{0}
        \end{cases}\\
        \implies &\begin{cases}
            \tilde{Q} &= Q^{-1} = Q^\top \\
            \tilde{\bm{d}} &= -\tilde{Q}\bm{d} = -Q^\top \bm{d}
        \end{cases}\\
        \implies T^{-1} &=\underline{ \begin{bmatrix}
            Q^\top & -Q^\top \bm{d} \\ \bm{0} & 1
        \end{bmatrix}
        }
    \end{aligned}
\end{equation}
\end{document}